src/varieties/setoid.v
@@ -54,4 +54,4 @@ Proof with try apply _.
  change (Algebra theory B)...
 Qed.
 
-Instance struct_from_var_to_class `{InVariety theory A}: Setoid (A tt).
+Instance decode_variety_and_ops `{InVariety theory A}: Setoid (A tt).
